Sources/WasmToBoogie/obj/Debug/net9.0/WasmToBoogie.AssemblyInfo.cs
@@ -13,7 +13,7 @@ using System.Reflection;
 [assembly: System.Reflection.AssemblyCompanyAttribute("WasmToBoogie")]
 [assembly: System.Reflection.AssemblyConfigurationAttribute("Debug")]
 [assembly: System.Reflection.AssemblyFileVersionAttribute("1.0.0.0")]
-[assembly: System.Reflection.AssemblyInformationalVersionAttribute("1.0.0+7ae954e4813d06fa90b3510acda2d2d8488774ae")]
+[assembly: System.Reflection.AssemblyInformationalVersionAttribute("1.0.0+cc8976ca6603e0248781f13a532a2f33bfd205ac")]
 [assembly: System.Reflection.AssemblyProductAttribute("WasmToBoogie")]
 [assembly: System.Reflection.AssemblyTitleAttribute("WasmToBoogie")]
 [assembly: System.Reflection.AssemblyVersionAttribute("1.0.0.0")]
