BoogieOutputs/boogiePrelude.bpl
@@ -1,30 +1,77 @@
 var $stack: [int]real;
 var $sp: int;
+var $tmp1:real;
+var $tmp2:real;
+var $tmp3:real;
 
-procedure push(val: real)
+function bool_to_real(b: bool): real;
+function real_to_bool(r: real): bool;
+function real_to_int(r: real): int;
+
+axiom (forall b: bool :: bool_to_real(b) == (if b then 1.0 else 0.0));
+axiom (forall r: real :: real_to_bool(r) == (r != 0.0));
+axiom (forall r: real :: real_to_int(r) >= 0);
+
+
+procedure {:inline 1} push(val: real);
   modifies $sp, $stack;
+  
+implementation push(val: real)
 {
   $stack[$sp] := val;
   $sp := $sp + 1;
 }
 
-procedure popToTmp1()
+procedure popToTmp1();
   modifies $sp, $stack, $tmp1;
-{
+  
+implementation popToTmp1()
+{  
+
   $sp := $sp - 1;
   $tmp1 := $stack[$sp];
 }
 
-procedure popToTmp2()
-  modifies $sp, $stack, $tmp1;
-{
+procedure popToTmp2();
+  modifies $sp, $stack, $tmp2;
+implementation popToTmp2()
+{ 
+
   $sp := $sp - 1;
   $tmp2 := $stack[$sp];
 }
 
-procedure popToTmp3()
-  modifies $sp, $stack, $tmp1;
-{
+procedure popToTmp3();
+  modifies $sp, $stack, $tmp3;
+implementation popToTmp3()
+{  
+
   $sp := $sp - 1;
   $tmp3 := $stack[$sp];
+}
+
+procedure pop();
+  modifies $sp;
+implementation pop()
+{
+  $sp := $sp - 1;
+}
+
+procedure BoogieEntry_simple();
+  modifies $tmp1 ,$tmp2 , $sp, $stack;
+
+implementation BoogieEntry_simple() 
+{
+// // Type AST non supportÃƒÂ© : RawInstructionNode
+// // Type AST non supportÃƒÂ© : RawInstructionNode
+call push(5.0);
+call push(2.0);
+call push(3.0);
+call popToTmp1();
+call popToTmp2();
+call push(($tmp2) + ($tmp1));
+call popToTmp1();
+call popToTmp2();
+call push(bool_to_real(($tmp2) == ($tmp1)));
+call pop();
 }
