BoogieOutputs/simple.bpl
@@ -1,18 +1,125 @@
-procedure BoogieEntry_simple();
-implementation BoogieEntry_simple()
+var $stack: [int]real;
+var $sp: int;
+var $tmp1: real;
+var $tmp2: real;
+var $tmp3: real;
+function bool_to_real(b: bool) returns (result: real);
+function real_to_bool(r: real) returns (result: bool);
+function real_to_int(r: real) returns (result: int);
+
+axiom(forall  b:bool ::  ((bool_to_real(b)) == (if b then (1) else (0))));
+
+axiom(forall  r:real ::  ((real_to_bool(r)) == ((r) != (0))));
+
+axiom(forall  r:real ::  ((real_to_int(r)) >= (0)));
+procedure {:inline true} push(val: real);
+modifies $sp;
+modifies $stack;
+implementation push(val: real)
 {
-// // Type AST non supporté : RawInstructionNode
-// // Type AST non supporté : RawInstructionNode
+$stack[$sp] := val;
+$sp := ($sp) + (1);
+}
+
+procedure popToTmp1();
+modifies $sp;
+modifies $stack;
+modifies $tmp1;
+implementation popToTmp1()
+{
+$sp := ($sp) - (1);
+$tmp1 := $stack[$sp];
+}
+
+procedure popToTmp2();
+modifies $sp;
+modifies $stack;
+modifies $tmp2;
+implementation popToTmp2()
+{
+$sp := ($sp) - (1);
+$tmp2 := $stack[$sp];
+}
+
+procedure popToTmp3();
+modifies $sp;
+modifies $stack;
+modifies $tmp3;
+implementation popToTmp3()
+{
+$sp := ($sp) - (1);
+$tmp3 := $stack[$sp];
+}
+
+procedure pop();
+modifies $sp;
+implementation pop()
+{
+$sp := ($sp) - (1);
+}
+
+procedure func_simple();
+modifies $tmp1;
+modifies $tmp2;
+modifies $sp;
+modifies $stack;
+implementation func_simple()
+{
+// skip: exit_1:
+// skip: start_2:
+// // unhandled raw instruction: $none_=>_none
+// skip: func_5:
+// skip: type_4:
+// // unhandled raw instruction: $temp
 call push(5);
-call push(2);
 call push(3);
 call popToTmp1();
 call popToTmp2();
 call push(($tmp2) + ($tmp1));
+call push(8);
 call popToTmp1();
 call popToTmp2();
 call push(bool_to_real(($tmp2) == ($tmp1)));
 call pop();
+call push(0);
+call popToTmp1();
+call push(bool_to_real(($tmp1) == (0)));
+call pop();
+call push(1);
+call popToTmp1();
+if (real_to_bool($tmp1)) {
+call push(2);
+call push(2);
+call popToTmp1();
+call popToTmp2();
+call push(bool_to_real(($tmp2) == ($tmp1)));
+call popToTmp1();
+if (real_to_bool($tmp1)) {
+call push(42);
+call pop();
+} else {
+call push(99);
+call pop();
+}
+call push(77);
+call pop();
+} else {
+call push(0);
+call popToTmp1();
+call push(bool_to_real(($tmp1) == (0)));
+call popToTmp1();
+if (real_to_bool($tmp1)) {
+call push(100);
+call pop();
+} else {
+call push(200);
+call pop();
+}
+call push(888);
+call pop();
+}
+// skip: func_6:
+// skip: module_3:
 }
 
 
